code/hpke/Hacl.HPKE.Curve64_CP128_SHA256.fsti
@@ -11,7 +11,7 @@ let cs = (DH.DH_Curve25519, AEAD.CHACHA20_POLY1305, Hash.SHA2_256)
 noextract unfold
 let vale_p = Vale.X64.CPU_Features_s.(adx_enabled /\ bmi2_enabled)
 
-val setupBaseI: setupBaseI_st cs vale_p
+val setupBaseS: setupBaseS_st cs vale_p
 
 val setupBaseR: setupBaseR_st cs vale_p
 
